Test Signature

code/experimental/pkcs11/Specification/PKCS11.Testing.Signature.fst
@@ -14,6 +14,24 @@ module L = PKCS11.Spec.Lemmas
 
 #set-options "--z3rlimit 300"
 
+
+(* Test0
+	Checks: correct 1-piecec sign
+	Expected result: passes
+	Result: passes
+
+	Test1: 
+	Checks: correct upd-fin sign
+	Expected result: passes
+	Result: passes
+
+	Test2: 
+	Checks: sign without init
+	Expected result: fails
+	Result: fails
+
+ *)
+
 val test0: d: device -> 
 	hSession: _CK_SESSION_HANDLE -> 
 	pMechanism: _CK_MECHANISM_TYPE{isPresentOnDevice d pMechanism /\ 
@@ -57,7 +75,7 @@ let test0 d hSession pMechanism keyHandler toSign lenToSign =
 	end	
 		
 
-val signature: d: device -> 
+val test1: d: device -> 
 	hSession: _CK_SESSION_HANDLE -> 
 	pMechanism: _CK_MECHANISM_TYPE{isPresentOnDevice d pMechanism /\ 
 		(let flags = mechanismGetFlags d pMechanism in isFlagSign flags)} ->
@@ -76,7 +94,7 @@ val signature: d: device ->
 	)
 	(ensures (fun h -> True))
 
-let signature d hSession pMechanism keyHandler toSign lenToSign = 
+let test1 d hSession pMechanism keyHandler toSign lenToSign = 
 	let len = 20 in 
 	let signaturePlace = Seq.create len 0uy in 
 
@@ -109,3 +127,38 @@ let signature d hSession pMechanism keyHandler toSign lenToSign =
 					end
 			else false		
 		end	
+
+
+
+val test2: d: device -> 
+	hSession: _CK_SESSION_HANDLE -> 
+	pMechanism: _CK_MECHANISM_TYPE{isPresentOnDevice d pMechanism /\ 
+		(let flags = mechanismGetFlags d pMechanism in isFlagSign flags)} ->
+	keyHandler: _CK_OBJECT_HANDLE{Seq.length d.keys > keyHandler /\ 
+		(let key = Seq.index d.keys keyHandler in 
+		let attrKey = (key.element).attrs in
+		isAttributeSign attrKey)} -> 
+	toSign: seq UInt8.t -> 
+	lenToSign: _CK_ULONG{Seq.length toSign = lenToSign} -> 	
+	Pure bool
+	(requires
+		(
+			let f = predicateSessionSignature hSession in 
+			let openedSessions = d.subSessions in L.count f openedSessions = 0
+		)
+	)
+	(ensures (fun h -> True))
+
+let test2 d hSession pMechanism keyHandler toSign lenToSign = 
+	let len = 20 in 
+	let signaturePlace = Seq.create len 0uy in 
+	let r = sign d hSession toSign lenToSign (Some signaturePlace) len in 
+	let deviceAfterSignature = dfst r in 
+	let  signature = dsnd r in 
+	match signature with 
+		|Inr a -> false 
+		|Inl v -> let (v, _) = v in 
+			match v with 
+			| None -> false
+			| Some b -> true
+		
